\begin{gather*}
        \nord{a(x)b(x')} = a(x)b(x') + b(x')a(x)
        \\
        \Tordp(a(x)b(x')) = \theta(t-'t)a(x)b(x') + \theta(t'-t)b(x')a(x)
\end{gather*}

The ``$+$'' corresponds to positive frequency plane waves $e^{-ik\cdot x}$:
\begin{gather*}
        \comm{\phi(\va{x},t)}{\phi(\va{y},t)} = \comm{\Pi(\va{x},t)}{\Pi(\va{y},t)} = 0
        \qquad
        \comm{\phi(\va{x},t)}{\Pi(\va{y},t)} = i\delta^3\qty(\va{x}-\va{y})
        \\
        \comm{a^\dagger\qty(k,\lambda)}{a\qty(k',\lambda')}
        = g^{\lambda\lambda'}\Tdelta\qty(k-k')
        \\
        A_\mu(x)
        = A_\mu^+(x) + A_\mu^-(x)
        = \int\Tdd{k}\sum_{\lambda=0}^3 \qty[a(k,\lambda)\epsilon_\mu(k,\lambda)e^{-ik\cdot x} + a^\dagger(k,\lambda)\epsilon_\mu^*(k,\lambda)e^{+ik\cdot x}]
        \\
        \ket{p} = a^\dagger(p)\ket{0}
        \qquad
        \ket{p_1,p_2} = a^\dagger(p_2)a^\dagger(p_1)\ket{0} = \ket{p_2,p_1}
        \\
        A^+(a) \text{ destroys } \ce{\gamma}
        \quad
        A^-(a^\dagger) \text{ creates } \ce{\gamma}
\end{gather*}

\begin{gather*}
        \comm{a_+(p)}{a_+^\dagger(q)}
        = \comm{a_-(p)}{a_-^\dagger(q)}
        = \Tdelta(p-q)
        \\
        \varphi(x)
        = \varphi^+(x) + \varphi^-(x)
        = \int\Tdd{k} \qty[a_+(k)e^{-ik\cdot x} + a_-^\dagger(k)e^{+ik\cdot x}]
        \\
        \varphi^\dagger(x)
        = \varphi^{+\dagger}(x) + \varphi^{-\dagger}(x)
        = \int\Tdd{k} \qty[a_-(k)e^{-ik\cdot x} + a_+^\dagger(k)e^{+ik\cdot x}]
        \\
        \ket{p^+} = a_+^\dagger(p)\ket{0}
        \qquad
        \ket{p^-} = a_-^\dagger(p)\ket{0}
        \qquad
        \ket{p_1^+,p_2^-} = a_-^\dagger(p_2)a_+^\dagger(p_1)\ket{0}
\end{gather*}
