\begin{gather*}
        \sigma_x = \begin{pmatrix}
                0 &1\\
                1 &0
        \end{pmatrix}
        \qquad
        \sigma_y = \begin{pmatrix}
                0 &-i\\
                i &0
        \end{pmatrix}
        \qquad
        \sigma_z = \begin{pmatrix}
                1 &0\\
                0 &-1
        \end{pmatrix}
        \qquad
        \va*{\Sigma} = \frac{1}{2}\begin{pmatrix}
                \va*{\sigma} &0\\
                0 &\va*{\sigma}\\
        \end{pmatrix}
        \\
        \va{S} = \frac{1}{2}\va*{\Sigma}
        \qquad
        \tilde{h}
        = \frac{\va{S}\vdot\va{p}}{\abs{\va{p}}}
        = \frac{\va*{\Sigma}\vdot\va{p}}{2\abs{\va{p}}}
        \qquad
        \tilde{h}
        = 2h
        = \frac{\va*{\Sigma}\vdot\va{p}}{\abs{\va{p}}}
        \qquad
        P_L = \frac{1 - h}{2}
        \qquad
        P_R = \frac{1 + h}{2}
        \\
        \gamma_L = \frac{1 - \gamma_5}{2}
        \qquad
        \gamma_R = \frac{1 + \gamma_5}{2}
        \qquad
        \gamma_{L,R}^2 = \gamma_{L,R}
        \qquad
        \gamma_{L,R}\gamma_{R,L} = 0
        \qquad
        \gamma_L + \gamma_R = \1
        \\
        \gamma^\mu\gamma_{L,R} = \gamma_{R,L}\gamma^\mu
        \qquad
        \gamma_5\gamma_{L} = \gamma_{L}\gamma_5 = -\gamma_{L}
        \qquad
        \gamma_5\gamma_{R} = \gamma_{R}\gamma_5 = \gamma_{R}
        \qquad
        \gamma_{L,R}^\dagger = \gamma_{L,R}
        \\
        \overline{\gamma^\mu\gamma_{L,R}} = \gamma^\mu\gamma_{L,R}
        \qquad
        \overline{\gamma_5\gamma_{L}} = -\gamma_{R}
        \qquad
        \overline{\gamma_5\gamma_{R}} = \gamma_{L}
        \qquad
        \overline{\gamma_{L,R}}
        = \gamma_0\gamma_{L,R}^\dagger\gamma_0
        = \gamma_{R,L}
\end{gather*}

\begin{gather*}
        u_L = u_\downarrow
        \qquad
        u_R = u_\uparrow
        \qquad
        v_L = v_\uparrow
        \qquad
        v_R = v_\downarrow
        \\
        \resizebox{\linewidth}{!}{$\displaystyle
                P_Lu_\downarrow = u_\downarrow
                \quad
                P_Lu_\uparrow = 0
                \qquad
                P_Ru_\downarrow = 0
                \quad
                P_Ru_\uparrow = u_\uparrow
                \qquad
                \overline{u_\downarrow}P_L = 0
                \quad
                \overline{u_\uparrow}P_L = u_\uparrow
                \qquad
                \overline{u_\downarrow}P_R = u_\downarrow
                \quad
                \overline{u_\uparrow}P_R = 0
        $}
        \\\resizebox{\linewidth}{!}{$\displaystyle
                \gamma_Lu_L = u_L
                \quad
                \gamma_Lu_R = 0
                \qquad
                \gamma_Ru_L = 0
                \quad
                \gamma_Ru_R = u_R
                \qquad
                \overline{u_L}\gamma_L = 0
                \quad
                \overline{u_R}\gamma_L = u_R
                \qquad
                \overline{u_L}\gamma_R = u_L
                \quad
                \overline{u_R}\gamma_R = 0
        $}
        \\\resizebox{\linewidth}{!}{$\displaystyle
                P_Lv_\downarrow = 0
                \quad
                P_Lv_\uparrow = v_\uparrow
                \qquad
                P_Rv_\downarrow = v_\downarrow
                \quad
                P_Rv_\uparrow = 0
                \qquad
                \overline{v_\downarrow}P_L = v_\downarrow
                \quad
                \overline{v_\uparrow}P_L = 0
                \qquad
                \overline{v_\downarrow}P_R = 0
                \quad
                \overline{v_\uparrow}P_R =v_\uparrow
        $}
        \\\resizebox{\linewidth}{!}{$\displaystyle
                \gamma_Lv_L = v_L
                \quad
                \gamma_Lv_R = 0
                \qquad
                \gamma_Rv_L = 0
                \quad
                \gamma_Rv_R = v_R
                \qquad
                \overline{v_L}\gamma_L = 0
                \quad
                \overline{v_R}\gamma_L = v_R
                \qquad
                \overline{v_L}\gamma_R = v_L
                \quad
                \overline{v_R}\gamma_R = 0
        $}
\end{gather*}

\begin{gather*}
        u_\uparrow = N \begin{pmatrix}
                c\\se^{i\phi}\\kc\\kse^{i\phi}
        \end{pmatrix}
        \approx N \begin{pmatrix}
                c\\se^{i\phi}\\c\\se^{i\phi}
        \end{pmatrix}\qquad
        u_\downarrow = N \begin{pmatrix}
                -s\\ce^{i\phi}\\ks\\-kce^{i\phi}
        \end{pmatrix}
        \approx N \begin{pmatrix}
                -s\\ce^{i\phi}\\s\\-ce^{i\phi}
        \end{pmatrix}
        \\
        v_\uparrow = N \begin{pmatrix}
                ks\\-kce^{i\phi}\\-s\\ce^{i\phi}
        \end{pmatrix}
        \approx N \begin{pmatrix}
                s\\-ce^{i\phi}\\-s\\ce^{i\phi}
        \end{pmatrix}\qquad
        v_\downarrow = N \begin{pmatrix}
                kc\\kse^{i\phi}\\c\\se^{i\phi}
        \end{pmatrix}
        \approx N \begin{pmatrix}
                c\\se^{i\phi}\\c\\se^{i\phi}
        \end{pmatrix}
        \\
        \va{p} = p\qty(\sin\theta\cos\phi , \sin\theta\sin\phi , \cos\theta)
        \\
        N = \sqrt{E+m} \approx \sqrt{E}
        \qquad
        k = \frac{p}{E+m} \approx 1
        \qquad
        s = \sin(\frac{\theta}{2})
        \qquad
        c = \cos(\frac{\theta}{2})
\end{gather*}
