\begin{gather*}
        i\hbar\pdv{\ket{\psi(t)}}{t} = H\ket{\psi(t)}
        \qquad\quad
        (\partial\cdot\partial + m^2)\phi = 0
        \qquad\quad
        \qty(i\slashed{\partial}-m)\varphi = 0
        \qquad
        \overline{\varphi}\qty(i\slashed{\partial}+m) = 0
        \\
        E = \qty(\va*{\alpha}\vdot\va{p} + \beta m)\varphi
        \implies
        i\pdv{\varphi}{t} = \qty(-i\va*{\alpha}\vdot\grad + \beta m)\varphi
        \implies
        \qty(i\gamma^\mu\partial_\mu - m)\varphi = \qty(i\gamma^\mu p_\mu - m)\varphi = 0
\end{gather*}
