\begin{gather*}
        \nord{a(x)b(x')} = a(x)b(x') - b(x')a(x)
        \\
        \Tordp(a(x)b(x')) = \theta(t-'t)a(x)b(x') - \theta(t'-t)b(x')a(x)
\end{gather*}
\begin{gather*}
        \acomm{b^\dagger\qty(p,s)}{b\qty(p',s')}
        = \acomm{d^\dagger\qty(p,s)}{d\qty(p',s')}
        = \Tdelta(p-p')\delta_{ss'}
        \\
        \psi(x)
        = \psi^+(x) + \psi^-(x)
        = \int\Tdd{p}\sum_s \qty[b(p,s)u(p,s)e^{-ip\cdot x} + d^\dagger(p,s)v(p,s)e^{+ip\cdot x}]
        \\
        \overline{\psi}(x)
        = \overline{\psi}^+(x) + \overline{\psi}^-(x)
        = \int\Tdd{p}\sum_s \qty[d(p,s)\overline{v}(p,s)e^{-ip\cdot x} + b^\dagger(p,s)\overline{u}(p,s)e^{+ip\cdot x}]
        \\
        \ket{e^-(p_1,s_1),e^-(p_2,s_2)} = b^\dagger(p_2,s_2)b^\dagger(p_1,s_1)\ket{0} = -\ket{e^-(p_2,s_2),e^-(p_1,s_1)}
        \\
        \psi^+(b) \text{ destroys } \ce{e^-}
        \quad
        \psi^-(d^\dagger) \text{ creates } \ce{e^+}
        \quad
        \overline{\psi}^+(d) \text{ destroy } \ce{e^+}
        \quad
        \overline{\psi}^-(b^\dagger) \text{ creates } \ce{e^-}
\end{gather*}
