\begin{gather*}
        \sigma^\mu=\qty(\mathbb{1},\va*{\sigma})
        \qquad
        \overline{\sigma}^\mu=\qty(\mathbb{1},-\va*{\sigma})
        \\
        \sigma^1 = \sigma_x = \begin{pmatrix}
                0 &1\\
                1 &0
        \end{pmatrix}
        \quad
        \sigma^2 = \sigma_y = \begin{pmatrix}
                0 &-i\\
                i &0
        \end{pmatrix}
        \quad
        \sigma^3 = \sigma_z = \begin{pmatrix}
                1 &0\\
                0 &-1
        \end{pmatrix}
        \quad
        \va*{\Sigma} = \begin{pmatrix}
                \va*{\sigma} &0\\
                0 &\va*{\sigma}\\
        \end{pmatrix}
        \\
        \acomm{\sigma^i}{\sigma^j} = 2\delta^{ij}
        \qquad
        \comm{\sigma^i}{\sigma^j} = 2i\epsilon^{ijk}\sigma^k
        \qquad
        \sigma^i\sigma^j = \delta^{ij} + i\epsilon^{ijk}\sigma^k
        \qquad
        \sigma^2\sigma^i\sigma^2 = -\qty(\sigma^i)^*
        \\
        \va*{\sigma}\vdot\va{p} = \begin{pmatrix}
                p_z      &p_x-ip_y \\
                p_x+ip_y &-p_z     \\
        \end{pmatrix}
        \qquad
        \qty(\va*{\sigma}\vdot\va{p})^2 = \abs{\va{p}}^2
        \qquad
        \qty(p\cdot\sigma)\qty(p\cdot\overline{\sigma}) = p^2
        \\
        p\cdot\overline{\sigma} = \begin{pmatrix}
                p^0+p^3  &p^1-ip^2 \\
                p^1+ip^2 &p^0-p^3  \\
        \end{pmatrix}
        \qquad
        p\cdot\sigma = \begin{pmatrix}
                p^0 - p^3       &-\qty(p^1-ip^2) \\
                -\qty(p^1+ip^2) &p^0+p^3         \\
        \end{pmatrix}
        \\
        \sqrt{p\cdot\sigma} = \frac{E + m - \va*{\sigma}\vdot\va{p}}{\sqrt{2(E+m)}}
        \qquad
        \sqrt{p\cdot\overline{\sigma}} = \frac{E + m + \va*{\sigma}\vdot\va{p}}{\sqrt{2(E+m)}}
\end{gather*}
