External massless \& Massive:
\begin{equation*}
        \sum_{\lambda=1}^{2} \epsilon^{\mu}(k,\lambda) \cdot \epsilon^{*\nu}(k,\lambda) = -g^{\mu\nu}
        \qquad
        \sum_{\lambda=1}^{3} \epsilon_\mu(q,\lambda)\epsilon^*_\nu(q,\lambda)
        = -g_{\mu\nu} + \frac{q_\mu q_\nu}{M^2}
\end{equation*}

%Virtual massless:
%\begin{equation*}
%        \epsilon(k,\lambda) \cdot \epsilon^*(k,\lambda') = g^{\lambda\lambda'}
%        \qquad
%        \sum_{\lambda}g^{\lambda\lambda} \epsilon^{\mu}(k,\lambda) \cdot \epsilon^{*\nu}(k,\lambda) = g^{\mu\nu}
%\end{equation*}
