\begin{gather*}
        \nord{\frac{1}{2}\qty[a^\dagger(k)a(k) + a(k)a^\dagger(k)]} = a^\dagger(k)a(k)
        \qquad
        \nord{a(x)b(x')} = a(x)b(x') + b(x')a(x)
        \\
        \Tordp(a(x)b(x')) = \theta(t-t')a(x)b(x') + \theta(t'-t)b(x')a(x)
\end{gather*}

The ``$+$'' corresponds to positive frequency plane waves $e^{-ik\cdot x}$:
\begin{gather*}
        \Lc = \frac{1}{2}\partial^\mu\phi\partial_\mu\phi - \frac{1}{2}m^2\phi\phi
        \qquad
        \pi = \dot{\phi}
        \qquad
        \comm{a^\dagger\qty(k,\lambda)}{a\qty(k',\lambda')}
        = g^{\lambda\lambda'}\Tdelta\qty(k-k')
        \\
        \comm{\phi(\va{x},t)}{\phi(\va{y},t)} = \comm{\Pi(\va{x},t)}{\Pi(\va{y},t)} = 0
        \qquad
        \comm{\phi(\va{x},t)}{\Pi(\va{y},t)} = i\delta^3\qty(\va{x}-\va{y})
        \\
        \phi(x) = \int\Tdd{k}\qty[a(k)e^{-ik\cdot x} + a^\dagger(k)e^{+ik\cdot x}]
        \\
        \ket{p} = a^\dagger(p)\ket{0}
        \qquad
        \ket{p_1,p_2} = a^\dagger(p_2)a^\dagger(p_1)\ket{0} = \ket{p_2,p_1}
\end{gather*}
