\begin{gather*}
        \Lc = -\frac{1}{4}F_{\mu\nu}F^{\mu\nu} - \frac{1}{2\xi}\qty(\partial\cdot A)^2
        \qquad
        %\pi^\mu = \pdv{\Lc}{\dot{A}_\mu} = F^{\mu0} - \frac{g^{\mu0}}{\xi}\qty(\partial\cdot A)
        \pi^\mu = F^{\mu0} - \frac{g^{\mu0}}{\xi}\qty(\partial\cdot A)
        \qquad
        \pi^0 = -\frac{1}{\xi}\qty(\partial\cdot A)
        \quad
        \pi^k = E^k
        \\
        \comm{A_\mu(\va{x},t)}{A_\nu(\va{y},t)}
        = \comm{\dot{A}_\mu(\va{x},t)}{\dot{A}_\nu(\va{y},t)}
        = 0
        \qquad
        \comm{\dot{A}_\mu(\va{y},t)}{A_\nu(\va{x},t)}
        = ig_{\mu\nu}\Ddelta[3](\va{x}-\va{y})
        \\
        A_\mu(x)
        = A_\mu^+(x) + A_\mu^-(x)
        = \int\Tdd{k} \sum_{\lambda=0}^3\qty[a(k,\lambda)\epsilon_\mu(k,\lambda)e^{-ik\cdot x} + a^\dagger(k,\lambda)\epsilon^*_\mu(k,\lambda)e^{+ik\cdot x}]
        \\
        \begin{aligned}
                A_\mu^+(x)\ket{k} = A_\mu^+(x)a^\dagger(k)\ket{0} = \ket{0}\epsilon_\mu(k)e^{-ik\cdot x}
                &\qquad
                \comm{\dot{a}(k,\lambda)}{a^\dagger(k',\lambda')}
                = - g^{\lambda\lambda'}\Tdelta(k-k')
                \\
                \bra{k}A_\mu^-(x) = \bra{0}a(k)A_\mu^-(x) = \epsilon^*_\mu(k)e^{+ik\cdot x}\bra{0}
                &\qquad
                A^+(a) \text{ destroys } \ce{\gamma}
                \quad
                A^-(a^\dagger) \text{ creates } \ce{\gamma}
        \end{aligned}
\end{gather*}
