\begin{gather*}
        \nord{a(x)b(x')} = a(x)b(x') - b(x')a(x)
        \\
        \Tordp(a(x)b(x')) = \theta(t-'t)a(x)b(x') - \theta(t'-t)b(x')a(x)
\end{gather*}

\begin{gather*}
        \Lc = \nord{i\overline{\psi}\gamma^\mu\partial_\mu\psi - m\overline{\psi}\psi}
        \qquad
        \pi_\alpha = \pdv{\Lc}{\dot{\psi_\alpha}} = i\psi_\alpha^\dagger
        \qquad
        \pi_\alpha^\dagger = \pdv{\Lc}{\dot{\psi_\alpha}^\dagger} = 0
        \\
        \acomm{b^\dagger\qty(p,s)}{b\qty(p',s')}
        = \acomm{d^\dagger\qty(p,s)}{d\qty(p',s')}
        = \Tdelta(p-p')\delta_{ss'}
        \\
        \psi(x)
        = \psi^+(x) + \psi^-(x)
        = \int\Tdd{p}\sum_s \qty[b(p,s)u(p,s)e^{-ip\cdot x} + d^\dagger(p,s)v(p,s)e^{+ip\cdot x}]
        \\
        \overline{\psi}(x)
        = \overline{\psi}^+(x) + \overline{\psi}^-(x)
        = \int\Tdd{p}\sum_s \qty[d(p,s)\overline{v}(p,s)e^{-ip\cdot x} + b^\dagger(p,s)\overline{u}(p,s)e^{+ip\cdot x}]
        \\
        \ket{e^-(p_1,s_1),e^-(p_2,s_2)} = b^\dagger(p_2,s_2)b^\dagger(p_1,s_1)\ket{0} = -\ket{e^-(p_2,s_2),e^-(p_1,s_1)}
        \\
        \begin{aligned}
                \psi^+(x)\ket{p} = \psi^+(x)b^\dagger(p)\ket{0} = \ket{0} u(p)e^{-ip\cdot x}
                &\qquad
                \psi^+(b) \text{ destroys } \ce{e^-}
                \\
                \overline{\psi}^+(x)\ket{p} = \overline{\psi}^+(x)d^\dagger(p)\ket{0} = \ket{0} \overline{v}(p)e^{-ip\cdot x}
                &\qquad
                \overline{\psi}^+(d) \text{ destroy } \ce{e^+}
                \\
                \bra{p}\psi^-(x) = \bra{0}d(p)\psi^-(x) = v(p)e^{+ip\cdot x}\bra{0}
                &\qquad
                \psi^-(d^\dagger) \text{ creates } \ce{e^+}
                \\
                \bra{p}\overline{\psi}^-(x) = \bra{0}b(p)\overline{\psi}^-(x) = \overline{u}(p)e^{+ip\cdot x}\bra{0}
                &\qquad
                \overline{\psi}^-(b^\dagger) \text{ creates } \ce{e^-}
        \end{aligned}
\end{gather*}
