\begin{gather*}
        \beta
        = \frac{v}{c}
        = \frac{p}{E}
        = \tanh(\eta)
        \qquad
        \gamma
        = \frac{1}{\sqrt{1-\beta^2}}
        = \cosh(\eta)
        \qquad
        \gamma\beta = \sin(\eta)
        \\
        E^2 = m^2 + \abs{p}^2
        \qquad
        \frac{\dd[3]{\va{p}'}}{E'} = \frac{\dd[3]{\va{p}}}{E}
\end{gather*}

\begin{gather*}
        x^{\mu} = (t, \va{x})
        \qquad
        p^{\mu} = (E, \va{p})
        \qquad
        \partial^{\mu} = \qty(\partial_t, -\va{\nabla})
        \qquad
        A^{\mu} = \qty(\phi, \va{A})
        \qquad
        J^{\mu} = \qty(\rho, \va{J})
        \\
        F^{\mu\nu} \equiv \partial^\mu A^\nu - \partial^\nu A^\mu
        \qquad
        \Fc^{\mu\nu} = \frac{1}{2}\epsilon^{\mu\nu\alpha\beta}F_{\alpha\beta}
        \qquad
        \partial_\mu F^{\mu\nu} = J^{\nu}
        \qquad
        \partial_\mu \Fc^{\mu\nu} = 0
\end{gather*}

\begin{equation*}
        \epsilon^{\mu\nu\rho\sigma} = \begin{cases}
                +1 &\text{If $(\mu\nu\rho\sigma)$ is an even permutation of $(0123)$} \\
                -1 &\text{If $(\mu\nu\rho\sigma)$ is an odd permutation of $(0123)$} \\
                0  &\text{Otherwise} \\
        \end{cases}
\end{equation*}

\begin{gather*}
    \begin{multlined}
        \epsilon_{\alpha\beta_1\gamma_1\delta_1}\epsilon^{\alpha\beta_2\gamma_2\delta_2}
        =
        + g^{\beta_2}_{\beta_1}g^{\delta_2}_{\gamma_1}g^{\gamma_2}_{\delta_1}
        - g^{\beta_2}_{\beta_1}g^{\gamma_2}_{\gamma_1}g^{\delta_2}_{\delta_1}
        + g^{\gamma_2}_{\beta_1}g^{\beta_2}_{\gamma_1}g^{\delta_2}_{\delta_1}
        - g^{\gamma_2}_{\beta_1}g^{\delta_2}_{\gamma_1}g^{\beta_2}_{\delta_1}
        \\
        + g^{\delta_2}_{\beta_1}g^{\gamma_2}_{\gamma_1}g^{\beta_2}_{\delta_1}
        - g^{\delta_2}_{\beta_1}g^{\beta_2}_{\gamma_1}g^{\gamma_2}_{\delta_1}
    \end{multlined}
    \\
    \epsilon_{\alpha\beta\gamma_1\delta_1}\epsilon^{\alpha\beta\gamma_2\delta_2} = -2\qty(g_{\gamma_1}^{\gamma_2}g_{\delta_1}^{\delta_2} - g_{\gamma_1}^{\delta_2}g_{\delta_1}^{\gamma_2})
    \qquad
    \epsilon_{\alpha\beta\gamma\delta_1}\epsilon^{\alpha\beta\gamma\delta_2} = -6g_{\delta_1}^{\delta_2}
\end{gather*}
