\begin{gather*}
        \dv{\sigma}{\Omega} = \frac{1}{64\pi^2s}\frac{\abs{\va{p}_{3}}}{\abs{\va{p}_{1}}}\overline{\abs{\Mc}^2}
        \qquad
        \abs{\va{p}_a} = \abs{\va{p}_b} = \frac{1}{2\sqrt{s}}\sqrt{\qty[s - (m_a+m_b)^2]\qty[s - \qty(m_a-m_b)^2]}
        \\
        E_1 = \frac{s + m_1^2 - m_2^2}{2\sqrt{s}}
        \quad
        E_2 = \frac{s + m_2^2 - m_1^2}{2\sqrt{s}}
        \quad
        E_3 = \frac{s + m_3^2 - m_4^2}{2\sqrt{s}}
        \quad
        E_4 = \frac{s + m_4^2 - m_3^2}{2\sqrt{s}}
\end{gather*}

\begin{align*}
        s
        &= (p_1 + p_2)^2 = (p_3 + p_4)^2
        \approx +2p_1\cdot p_2 \approx +2p_3\cdot p_4
        &&
        \sqrt{s} = E_{CM}
        \\
        t
        &= (p_1 - p_3)^2 = (p_2 - p_4)^2
        \approx -2p_1\cdot p_3 \approx -2p_2\cdot p_4
        &&
        s + t + u = m_1^2 + m_2^2 + m_3^2 + m_4^2
        \\
        u
        &= (p_1 - p_4)^2 = (p_2 - p_3)^2
        \approx -2p_1\cdot p_4 \approx -2p_2\cdot p_3
\end{align*}

\begin{gather*}
        \ce{f + $\overline{\mathrm{f}}$ -> g + $\overline{\mathrm{g}}$}:
        \qquad
        p_1 = \frac{\sqrt{s}}{2}\qty(1, 0, 0, +\beta_f)
        \qquad
        p_2 = \frac{\sqrt{s}}{2}\qty(1, 0, 0, -\beta_f)
        \\
        p_3 = \frac{\sqrt{s}}{2}\qty(1, +\beta_g\sin\theta, 0, +\beta_g\cos\theta)
        \qquad
        p_4 = \frac{\sqrt{s}}{2}\qty(1, -\beta_g\sin\theta, 0, -\beta_g\cos\theta)
\end{gather*}

\begin{equation*}
        m=0
        :\qquad
        s
        = 2\abs{\va{p}_{\mathrm{CM}}}^2
        = 2\qty(p^0_{\mathrm{CM}})^2
        \qquad
        t = -\frac{s}{2}\qty(1 - \cos\theta)
        \qquad
        u = -\frac{s}{2}\qty(1 + \cos\theta)
\end{equation*}
