\begin{gather*}
        \psi
        = ue^{+i\qty(\va{p}\vdot\va{x} - E\cdot t)}
        = ve^{-i\qty(\va{p}\vdot\va{x} - E\cdot t)}
        \qquad
        \qty(\slashed{p}-m)u
        = \overline{u}\qty(\slashed{p}-m)
        = 0
        =
        \qty(\slashed{p}+m)v
        = \overline{v}\qty(\slashed{p}+m)
        \\
        \overline{u}^r(p)u^s(p) = +2m\delta^{rs}
        \quad
        \overline{u}^r(p)v^s(p) = 0
        \quad
        u^{r\dagger}(p)u^s(p) = 2E\delta^{rs}
        \quad
        \sum_{s=1,2}u^s(p)\overline{u}^s(p) = \slashed{p} + m
        \\
        \overline{v}^r(p)v^s(p) = -2m\delta^{rs}
        \quad
        \overline{v}^r(p)u^s(p) = 0
        \quad
        v^{r\dagger}(p)v^s(p) = 2E\delta^{rs}
        \quad
        \sum_{s=1,2}v^s(p)\overline{v}^s(p) = \slashed{p} - m
\end{gather*}

\begin{equation*}
        m=0:
        \sum_{\lambda=1}^{2} \epsilon^{\mu}(k,\lambda) \cdot \epsilon^{*\nu}(k,\lambda) = -g^{\mu\nu}
        \qquad
        m\neq0:
        \sum_{\lambda=1}^{3} \epsilon_\mu(q,\lambda)\epsilon^*_\nu(q,\lambda)
        = -g_{\mu\nu} + \frac{q_\mu q_\nu}{M^2}
\end{equation*}
