\begin{gather*}
        \begin{alignedat}{3}
                &\Tr[\1] = 4
                \qquad
                &&\mathrm{Tr}[\underbrace{\gamma^\mu\gamma^\nu\dots\gamma^\rho}_{\mathclap{\text{Odd Number}}}] = 0
                \qquad
                &&\Tr[\gamma^\mu\gamma^\nu] = 4g^{\mu\nu}
                \\
                &\Tr[\gamma_5] = 0
                \qquad
                &&\mathrm{Tr}[\gamma_5\underbrace{\gamma^\mu\gamma^\nu\dots\gamma^\rho}_{\mathclap{\text{Odd Number}}}] = 0
                \qquad
                &&\Tr[\gamma_5\gamma^\mu\gamma^\nu] = 0
        \end{alignedat}
        \\
        \Tr[\gamma^\mu\gamma^\nu\gamma^\rho\gamma^\sigma] = 4\qty(g^{\mu\nu}g^{\rho\sigma} - g^{\mu\rho}g^{\nu\sigma} + g^{\mu\sigma}g^{\nu\rho})
        \qquad
        \Tr[\gamma_5\gamma^\mu\gamma^\nu\gamma^\rho\gamma^\sigma] = -4i\epsilon^{\mu\nu\rho\sigma}
        \\
        \Tr[\gamma^\mu\gamma^\nu\gamma^\rho\gamma^\sigma\gamma_L] = 2\qty(g^{\mu\nu}g^{\rho\sigma} - g^{\mu\rho}g^{\nu\sigma} + g^{\mu\sigma}g^{\nu\rho} + i\epsilon^{\mu\nu\rho\sigma})
        \\
        \Tr[\gamma^\mu\gamma^\nu\gamma^\rho\gamma^\sigma\gamma_R] = 2\qty(g^{\mu\nu}g^{\rho\sigma} - g^{\mu\rho}g^{\nu\sigma} + g^{\mu\sigma}g^{\nu\rho} - i\epsilon^{\mu\nu\rho\sigma})
\end{gather*}
\begin{equation*}
        \Tr[\qty(\slashed{p_a}+m_a)\gamma^\mu\qty(\slashed{p_b}+m_b)\gamma^\nu]
        = 4\qty[p_a^{\mu}p_b^{\nu} + p_b^{\mu}p_a^{\nu} + \qty(m_am_b - p_a\cdot p_b)g^{\mu\nu}]
\end{equation*}
